<?xml version="1.0"?>
<rdf:RDF xmlns="http://purl.org/he/syllabus/ontology#"
     xml:base="http://purl.org/he/syllabus/ontology"
     xmlns:os="http://purl.org/he/syllabus/ontology#"
     xmlns:ti="http://www.ontologydesignpatterns.org/cp/owl/timeinterval.owl#"
     xmlns:dct="http://purl.org/dc/terms/"
     xmlns:owl="http://www.w3.org/2002/07/owl#"
     xmlns:pro="http://purl.org/spar/pro/"
     xmlns:rdf="http://www.w3.org/1999/02/22-rdf-syntax-ns#"
     xmlns:tvc="http://www.essepuntato.it/2012/04/tvc/"
     xmlns:xml="http://www.w3.org/XML/1998/namespace"
     xmlns:xsd="http://www.w3.org/2001/XMLSchema#"
     xmlns:foaf="http://xmlns.com/foaf/0.1/"
     xmlns:frbr="http://purl.org/vocab/frbr/core#"
     xmlns:ieee="http://www.teste/ontologies/IEEE_RCD_Impl.owl"
     xmlns:rdfs="http://www.w3.org/2000/01/rdf-schema#"
     xmlns:skos="http://www.w3.org/2004/02/skos/core#"
     xmlns:time="http://www.w3.org/2006/time#"
     xmlns:vivo="http://vivoweb.org/ontology/core#"
     xmlns:aiiso="http://purl.org/vocab/aiiso/schema#"
     xmlns:fabio="http://purl.org/spar/fabio/"
     xmlns:sicra="http://www.fonte-project.net/ontologies/SICRA.owl"
     xmlns:teach="http://linkedscience.org/teach/ns#"
     xmlns:schema="http://schema.org/">
    <owl:Ontology rdf:about="http://purl.org/he/syllabus/ontology#">
        <dct:contributor>Janneth Chicaiza</dct:contributor>
        <dct:creator>Mariela Tapia-Leon</dct:creator>
        <dct:rights>This work is distribution under a Creative Commons Atribution License (https://creativecommons.org/licenses/by/4.0/legalcode)</dct:rights>
        <rdfs:comment xml:lang="en">Syllabus ontology provide a consensual knowledge model of syllabus domain. This model is a compilation of the main terms and objects for this particular domain and could be used by Higher Education Institutes.</rdfs:comment>
        <rdfs:label>Syllabus ontology</rdfs:label>
        <owl:versionInfo rdf:datatype="http://www.w3.org/2001/XMLSchema#decimal">1.4</owl:versionInfo>
    </owl:Ontology>
    


    <!-- 
    ///////////////////////////////////////////////////////////////////////////////////////
    //
    // Annotation properties
    //
    ///////////////////////////////////////////////////////////////////////////////////////
     -->

    


    <!-- http://purl.org/dc/terms/contributor -->

    <owl:AnnotationProperty rdf:about="http://purl.org/dc/terms/contributor"/>
    


    <!-- http://purl.org/dc/terms/creator -->

    <owl:AnnotationProperty rdf:about="http://purl.org/dc/terms/creator"/>
    


    <!-- http://purl.org/dc/terms/rights -->

    <owl:AnnotationProperty rdf:about="http://purl.org/dc/terms/rights"/>
    


    <!-- 
    ///////////////////////////////////////////////////////////////////////////////////////
    //
    // Object Properties
    //
    ///////////////////////////////////////////////////////////////////////////////////////
     -->

    


    <!-- http://linkedscience.org/teach/ns#studyProgram -->

    <owl:ObjectProperty rdf:about="http://linkedscience.org/teach/ns#studyProgram">
        <rdfs:domain rdf:resource="http://linkedscience.org/teach/ns#Course"/>
        <rdfs:range rdf:resource="http://purl.org/he/syllabus/ontology#Syllabus"/>
        <rdfs:comment>Describes the study program which is associated with the course/seminar.</rdfs:comment>
        <rdfs:label>study program</rdfs:label>
        <rdfs:label>syllabus</rdfs:label>
    </owl:ObjectProperty>
    


    <!-- http://linkedscience.org/teach/ns#teacher -->

    <owl:ObjectProperty rdf:about="http://linkedscience.org/teach/ns#teacher">
        <rdfs:domain rdf:resource="http://linkedscience.org/teach/ns#Course"/>
        <rdfs:range rdf:resource="http://linkedscience.org/teach/ns#Teacher"/>
        <rdfs:comment>Teacher is an abstract property to relate a teacher to a course/seminar.</rdfs:comment>
        <rdfs:label>teacher</rdfs:label>
    </owl:ObjectProperty>
    


    <!-- http://purl.org/dc/terms/creator -->

    <owl:ObjectProperty rdf:about="http://purl.org/dc/terms/creator">
        <owl:equivalentProperty rdf:resource="http://schema.org/creator"/>
        <rdfs:domain rdf:resource="http://purl.org/he/syllabus/ontology#Instructor"/>
        <rdfs:range rdf:resource="http://purl.org/he/syllabus/ontology#Syllabus"/>
    </owl:ObjectProperty>
    


    <!-- http://purl.org/dc/terms/language -->

    <owl:ObjectProperty rdf:about="http://purl.org/dc/terms/language">
        <rdfs:domain rdf:resource="http://schema.org/CourseInstance"/>
        <rdfs:range rdf:resource="http://purl.org/dc/terms/LinguisticSystem"/>
        <rdfs:comment>A language of the resource.</rdfs:comment>
        <rdfs:label>language</rdfs:label>
    </owl:ObjectProperty>
    


    <!-- http://purl.org/dc/terms/tableOfContents -->

    <owl:ObjectProperty rdf:about="http://purl.org/dc/terms/tableOfContents">
        <rdfs:domain rdf:resource="http://purl.org/he/syllabus/ontology#Syllabus"/>
        <rdfs:range rdf:resource="http://purl.org/he/syllabus/ontology#Content"/>
        <rdfs:comment>A list of subunits of the resource.</rdfs:comment>
        <rdfs:label>table of contents</rdfs:label>
    </owl:ObjectProperty>
    


    <!-- http://purl.org/he/syllabus/ontology#academicDegree -->

    <owl:ObjectProperty rdf:about="http://purl.org/he/syllabus/ontology#academicDegree">
        <rdfs:domain>
            <owl:Class>
                <owl:intersectionOf rdf:parseType="Collection">
                    <rdf:Description rdf:about="http://schema.org/Course"/>
                    <rdf:Description rdf:about="http://xmlns.com/foaf/0.1/Person"/>
                </owl:intersectionOf>
            </owl:Class>
        </rdfs:domain>
        <rdfs:range rdf:resource="http://vivoweb.org/ontology/core#AcademicDegree"/>
        <rdfs:comment>An academic degree at any level, both as reported by individuals for employment and as offered by academic degree programs.</rdfs:comment>
        <rdfs:label>academic degree</rdfs:label>
    </owl:ObjectProperty>
    


    <!-- http://purl.org/he/syllabus/ontology#academicTerm -->

    <owl:ObjectProperty rdf:about="http://purl.org/he/syllabus/ontology#academicTerm">
        <rdfs:domain rdf:resource="http://schema.org/CourseInstance"/>
        <rdfs:range rdf:resource="http://vivoweb.org/ontology/core#AcademicTerm"/>
        <rdfs:comment>An explicit individual academic term, quarter, or semester rather than the generic fall, spring or summer semester.</rdfs:comment>
        <rdfs:label>academic term</rdfs:label>
    </owl:ObjectProperty>
    


    <!-- http://purl.org/he/syllabus/ontology#academicYear -->

    <owl:ObjectProperty rdf:about="http://purl.org/he/syllabus/ontology#academicYear">
        <rdfs:domain rdf:resource="http://schema.org/CourseInstance"/>
        <rdfs:range rdf:resource="http://vivoweb.org/ontology/core#AcademicYear"/>
        <rdfs:comment>An explicit individual period considered by an academic institution to be its primary academic cycle.</rdfs:comment>
        <rdfs:label>academic year</rdfs:label>
    </owl:ObjectProperty>
    


    <!-- http://purl.org/he/syllabus/ontology#approve -->

    <owl:ObjectProperty rdf:about="http://purl.org/he/syllabus/ontology#approve">
        <rdfs:domain rdf:resource="http://purl.org/he/syllabus/ontology#Reviewer"/>
        <rdfs:range rdf:resource="http://purl.org/he/syllabus/ontology#Syllabus"/>
        <rdfs:comment>Entity who approves the syllabus.</rdfs:comment>
        <rdfs:label>approved</rdfs:label>
    </owl:ObjectProperty>
    


    <!-- http://purl.org/he/syllabus/ontology#assessment -->

    <owl:ObjectProperty rdf:about="http://purl.org/he/syllabus/ontology#assessment">
        <rdfs:domain>
            <owl:Class>
                <owl:intersectionOf rdf:parseType="Collection">
                    <rdf:Description rdf:about="http://purl.org/he/syllabus/ontology#Syllabus"/>
                    <rdf:Description rdf:about="http://purl.org/he/syllabus/ontology#Topic"/>
                </owl:intersectionOf>
            </owl:Class>
        </rdfs:domain>
        <rdfs:range rdf:resource="http://purl.org/he/syllabus/ontology#Assessment"/>
        <rdfs:comment>An evaluation to decide the quality or importance of something.</rdfs:comment>
        <rdfs:label>assessment</rdfs:label>
    </owl:ObjectProperty>
    


    <!-- http://purl.org/he/syllabus/ontology#assignment -->

    <owl:ObjectProperty rdf:about="http://purl.org/he/syllabus/ontology#assignment">
        <rdfs:domain>
            <owl:Class>
                <owl:intersectionOf rdf:parseType="Collection">
                    <rdf:Description rdf:about="http://purl.org/he/syllabus/ontology#Syllabus"/>
                    <rdf:Description rdf:about="http://purl.org/he/syllabus/ontology#Topic"/>
                </owl:intersectionOf>
            </owl:Class>
        </rdfs:domain>
        <rdfs:range rdf:resource="http://linkedscience.org/teach/ns#Assignment"/>
        <rdfs:comment>A piece of work given to someone, typically as part of their studies.</rdfs:comment>
        <rdfs:label>assignment</rdfs:label>
    </owl:ObjectProperty>
    


    <!-- http://purl.org/he/syllabus/ontology#awardedBy -->

    <owl:ObjectProperty rdf:about="http://purl.org/he/syllabus/ontology#awardedBy">
        <rdfs:domain rdf:resource="http://vivoweb.org/ontology/core#AcademicDegree"/>
        <rdfs:range rdf:resource="http://schema.org/EducationalOrganization"/>
        <rdfs:comment>Academic degree awared by an educational institution.</rdfs:comment>
        <rdfs:label>awared</rdfs:label>
    </owl:ObjectProperty>
    


    <!-- http://purl.org/he/syllabus/ontology#classroom -->

    <owl:ObjectProperty rdf:about="http://purl.org/he/syllabus/ontology#classroom">
        <rdfs:domain rdf:resource="http://schema.org/CourseInstance"/>
        <rdfs:range rdf:resource="http://purl.org/he/syllabus/ontology#Classroom"/>
        <rdfs:comment>A room in an educational intitution where groups of students are taught.</rdfs:comment>
        <rdfs:label>classroom</rdfs:label>
    </owl:ObjectProperty>
    


    <!-- http://purl.org/he/syllabus/ontology#goal -->

    <owl:ObjectProperty rdf:about="http://purl.org/he/syllabus/ontology#goal">
        <rdfs:domain rdf:resource="http://purl.org/he/syllabus/ontology#Syllabus"/>
        <rdfs:range rdf:resource="http://purl.org/he/syllabus/ontology#GoalStatement"/>
        <rdfs:comment>The goal statement is one of the most important parts of the definition syllabus. With clearly and concisely stated goals, the rest of the planning process falls naturally into place.</rdfs:comment>
        <rdfs:label>goal</rdfs:label>
    </owl:ObjectProperty>
    


    <!-- http://purl.org/he/syllabus/ontology#hasSchedule -->

    <owl:ObjectProperty rdf:about="http://purl.org/he/syllabus/ontology#hasSchedule">
        <rdfs:domain>
            <owl:Class>
                <owl:intersectionOf rdf:parseType="Collection">
                    <rdf:Description rdf:about="http://purl.org/he/syllabus/ontology#Instructor"/>
                    <rdf:Description rdf:about="http://schema.org/CourseInstance"/>
                </owl:intersectionOf>
            </owl:Class>
        </rdfs:domain>
        <rdfs:range rdf:resource="http://purl.org/he/syllabus/ontology#Schedule"/>
        <rdfs:comment>Schedule of the class, laboratory, tutoring, etc.</rdfs:comment>
        <rdfs:label>schedule</rdfs:label>
    </owl:ObjectProperty>
    


    <!-- http://purl.org/he/syllabus/ontology#help -->

    <owl:ObjectProperty rdf:about="http://purl.org/he/syllabus/ontology#help">
        <rdfs:domain rdf:resource="http://purl.org/he/syllabus/ontology#Syllabus"/>
        <rdfs:range rdf:resource="http://purl.org/he/syllabus/ontology#Help"/>
        <rdfs:comment>Information or advice given to reach success in a course</rdfs:comment>
        <rdfs:label>help</rdfs:label>
    </owl:ObjectProperty>
    


    <!-- http://purl.org/he/syllabus/ontology#learningResource -->

    <owl:ObjectProperty rdf:about="http://purl.org/he/syllabus/ontology#learningResource">
        <rdfs:domain rdf:resource="http://purl.org/he/syllabus/ontology#Syllabus"/>
        <rdfs:range rdf:resource="dct:BibliographicResource"/>
        <rdfs:comment>List of resources of the course.</rdfs:comment>
        <rdfs:label>learning resources</rdfs:label>
    </owl:ObjectProperty>
    


    <!-- http://purl.org/he/syllabus/ontology#methodology -->

    <owl:ObjectProperty rdf:about="http://purl.org/he/syllabus/ontology#methodology">
        <rdfs:domain rdf:resource="http://purl.org/he/syllabus/ontology#Syllabus"/>
        <rdfs:range rdf:resource="http://purl.org/he/syllabus/ontology#Methodology"/>
        <rdfs:comment>A system of ways of doing, teaching, or studying something.</rdfs:comment>
        <rdfs:label>methodology</rdfs:label>
    </owl:ObjectProperty>
    


    <!-- http://purl.org/he/syllabus/ontology#policy -->

    <owl:ObjectProperty rdf:about="http://purl.org/he/syllabus/ontology#policy">
        <rdfs:domain rdf:resource="http://purl.org/he/syllabus/ontology#Syllabus"/>
        <rdfs:range rdf:resource="http://purl.org/he/syllabus/ontology#Policy"/>
        <rdfs:comment>Education policy are the principles and government policy-making in the educational sphere.</rdfs:comment>
        <rdfs:label>policy</rdfs:label>
    </owl:ObjectProperty>
    


    <!-- http://purl.org/he/syllabus/ontology#taxon -->

    <owl:ObjectProperty rdf:about="http://purl.org/he/syllabus/ontology#taxon">
        <rdfs:domain rdf:resource="http://purl.org/he/syllabus/ontology#GoalStatement"/>
        <rdfs:range rdf:resource="http://www.fonte-project.net/ontologies/SICRA.owlTaxonomiaBloom"/>
        <rdfs:comment>Bloom’s Taxonomy is a classification of the different objectives and skills that educators set for their students (learning objectives).</rdfs:comment>
        <rdfs:label>Bloom taxonomy</rdfs:label>
    </owl:ObjectProperty>
    


    <!-- http://purl.org/he/syllabus/ontology#workload -->

    <owl:ObjectProperty rdf:about="http://purl.org/he/syllabus/ontology#workload">
        <rdfs:domain rdf:resource="http://purl.org/he/syllabus/ontology#Syllabus"/>
        <rdfs:range rdf:resource="http://purl.org/he/syllabus/ontology#Workload"/>
        <rdfs:comment>The amount of work or of working time expected or assigned to do an activity.</rdfs:comment>
        <rdfs:label>workload</rdfs:label>
    </owl:ObjectProperty>
    


    <!-- http://purl.org/spar/fabio/hasManifestation -->

    <owl:ObjectProperty rdf:about="http://purl.org/spar/fabio/hasManifestation">
        <rdfs:domain rdf:resource="http://purl.org/vocab/frbr/core#Work"/>
        <rdfs:range rdf:resource="http://purl.org/vocab/frbr/core#Manifestation"/>
        <rdfs:comment>A property linking a particular work to its manifestations</rdfs:comment>
        <rdfs:label>has manifestation</rdfs:label>
    </owl:ObjectProperty>
    


    <!-- http://purl.org/spar/pro/holdsRoleInTime -->

    <owl:ObjectProperty rdf:about="http://purl.org/spar/pro/holdsRoleInTime">
        <rdfs:domain rdf:resource="http://xmlns.com/foaf/0.1/Agent"/>
        <rdfs:range rdf:resource="http://purl.org/spar/pro/RoleInTime"/>
        <rdfs:comment>A property relating an agent to a role that the agent holds.</rdfs:comment>
        <rdfs:label>holds role in time</rdfs:label>
    </owl:ObjectProperty>
    


    <!-- http://purl.org/spar/pro/withRole -->

    <owl:ObjectProperty rdf:about="http://purl.org/spar/pro/withRole">
        <rdfs:domain rdf:resource="http://purl.org/spar/pro/RoleInTime"/>
        <rdfs:range rdf:resource="http://purl.org/spar/pro/Role"/>
        <rdfs:comment>An object property connecting an agent&apos;s role in time to a definition of the type of role held by this agent, specified as an instance of the class pro:Role or of one of its sub-classes.</rdfs:comment>
        <rdfs:label>with role</rdfs:label>
    </owl:ObjectProperty>
    


    <!-- http://purl.org/vocab/aiiso/schema#part_of -->

    <owl:ObjectProperty rdf:about="http://purl.org/vocab/aiiso/schema#part_of">
        <rdfs:domain rdf:resource="http://schema.org/Organization"/>
        <rdfs:range rdf:resource="http://schema.org/Organization"/>
        <rdfs:comment>A foaf Organization may refer to its parent Organizations using part_of.</rdfs:comment>
        <rdfs:label>part of</rdfs:label>
    </owl:ObjectProperty>
    


    <!-- http://purl.org/vocab/frbr/core#embodiment -->

    <owl:ObjectProperty rdf:about="http://purl.org/vocab/frbr/core#embodiment">
        <rdfs:domain rdf:resource="http://purl.org/vocab/frbr/core#Expression"/>
        <rdfs:range rdf:resource="http://purl.org/vocab/frbr/core#Manifestation"/>
        <rdfs:comment>An expression embodied in a manifestation.</rdfs:comment>
        <rdfs:label>embodiment</rdfs:label>
    </owl:ObjectProperty>
    


    <!-- http://purl.org/vocab/frbr/core#realization -->

    <owl:ObjectProperty rdf:about="http://purl.org/vocab/frbr/core#realization">
        <rdfs:domain rdf:resource="http://purl.org/vocab/frbr/core#Work"/>
        <rdfs:range rdf:resource="http://purl.org/vocab/frbr/core#Expression"/>
        <rdfs:comment>A work realized through an expression</rdfs:comment>
        <rdfs:label>realization</rdfs:label>
    </owl:ObjectProperty>
    


    <!-- http://schema.org/audience -->

    <owl:ObjectProperty rdf:about="http://schema.org/audience">
        <rdfs:domain rdf:resource="http://schema.org/Course"/>
        <rdfs:range rdf:resource="http://schema.org/Audience"/>
        <rdfs:comment>Intended audience for an item, i.e. the group for whom the item was created.</rdfs:comment>
        <rdfs:label>audience</rdfs:label>
    </owl:ObjectProperty>
    


    <!-- http://schema.org/coursePrerequisites -->

    <owl:ObjectProperty rdf:about="http://schema.org/coursePrerequisites">
        <owl:equivalentProperty rdf:resource="http://vivoweb.org/ontology/core#hasPrerequisite"/>
        <rdfs:domain rdf:resource="http://schema.org/Course"/>
        <rdfs:range rdf:resource="http://schema.org/Course"/>
        <rdfs:comment>Requirements for taking the Course.</rdfs:comment>
        <rdfs:label>prerequisite</rdfs:label>
    </owl:ObjectProperty>
    


    <!-- http://schema.org/creator -->

    <owl:ObjectProperty rdf:about="http://schema.org/creator">
        <rdfs:domain rdf:resource="http://purl.org/he/syllabus/ontology#Instructor"/>
        <rdfs:range rdf:resource="http://purl.org/he/syllabus/ontology#Syllabus"/>
        <rdfs:comment>The creator/author of this CreativeWork. This is the same as the Author property for CreativeWork.</rdfs:comment>
        <rdfs:label>creator</rdfs:label>
    </owl:ObjectProperty>
    


    <!-- http://schema.org/hasCourseInstance -->

    <owl:ObjectProperty rdf:about="http://schema.org/hasCourseInstance">
        <rdfs:domain rdf:resource="http://schema.org/Course"/>
        <rdfs:range rdf:resource="http://schema.org/CourseInstance"/>
        <rdfs:comment>An offering of the course at a specific time and place or through specific media or mode of study or to a specific section of students.</rdfs:comment>
        <rdfs:label>course instance</rdfs:label>
    </owl:ObjectProperty>
    


    <!-- http://schema.org/instructor -->

    <owl:ObjectProperty rdf:about="http://schema.org/instructor">
        <rdfs:domain rdf:resource="http://schema.org/CourseInstance"/>
        <rdfs:range rdf:resource="http://purl.org/he/syllabus/ontology#Instructor"/>
        <rdfs:comment>A person assigned to instruct or provide instructional assistance for the CourseInstance.</rdfs:comment>
        <rdfs:label>instructor</rdfs:label>
        <rdfs:label>professor</rdfs:label>
    </owl:ObjectProperty>
    


    <!-- http://vivoweb.org/ontology/core#hasPrerequisite -->

    <owl:ObjectProperty rdf:about="http://vivoweb.org/ontology/core#hasPrerequisite">
        <rdfs:domain rdf:resource="http://vivoweb.org/ontology/core#Course"/>
        <rdfs:range rdf:resource="http://vivoweb.org/ontology/core#Course"/>
        <rdfs:comment>The prerequisites for taking the course.</rdfs:comment>
        <rdfs:label>prerequisite</rdfs:label>
    </owl:ObjectProperty>
    


    <!-- http://www.essepuntato.it/2012/04/tvc/atTime -->

    <owl:ObjectProperty rdf:about="http://www.essepuntato.it/2012/04/tvc/atTime">
        <rdfs:domain>
            <owl:Class>
                <owl:intersectionOf rdf:parseType="Collection">
                    <rdf:Description rdf:about="http://purl.org/he/syllabus/ontology#Schedule"/>
                    <rdf:Description rdf:about="http://purl.org/spar/pro/RoleInTime"/>
                    <rdf:Description rdf:about="http://schema.org/CourseInstance"/>
                </owl:intersectionOf>
            </owl:Class>
        </rdfs:domain>
        <rdfs:range rdf:resource="http://www.ontologydesignpatterns.org/cp/owl/timeinterval.owl#TimeInterval"/>
        <rdfs:comment>time of the event</rdfs:comment>
        <rdfs:label>at Time</rdfs:label>
    </owl:ObjectProperty>
    


    <!-- http://www.w3.org/2004/02/skos/core#member -->

    <owl:ObjectProperty rdf:about="http://www.w3.org/2004/02/skos/core#member">
        <rdfs:domain rdf:resource="http://www.w3.org/2004/02/skos/core#Collection"/>
        <rdfs:range>
            <owl:Class>
                <owl:intersectionOf rdf:parseType="Collection">
                    <rdf:Description rdf:about="http://www.w3.org/2004/02/skos/core#Collection"/>
                    <rdf:Description rdf:about="http://www.w3.org/2004/02/skos/core#Concept"/>
                </owl:intersectionOf>
            </owl:Class>
        </rdfs:range>
        <rdfs:comment>Collection has member</rdfs:comment>
        <rdfs:label>has member</rdfs:label>
    </owl:ObjectProperty>
    


    <!-- http://xmlns.com/foaf/0.1/member -->

    <owl:ObjectProperty rdf:about="http://xmlns.com/foaf/0.1/member">
        <rdfs:domain rdf:resource="http://schema.org/Person"/>
        <rdfs:range rdf:resource="http://schema.org/Organization"/>
        <rdfs:comment>Indicates a member of a Group.</rdfs:comment>
        <rdfs:label>member of a group</rdfs:label>
    </owl:ObjectProperty>
    


    <!-- 
    ///////////////////////////////////////////////////////////////////////////////////////
    //
    // Data properties
    //
    ///////////////////////////////////////////////////////////////////////////////////////
     -->

    


    <!-- http://purl.org/dc/terms/description -->

    <owl:DatatypeProperty rdf:about="http://purl.org/dc/terms/description">
        <owl:equivalentProperty rdf:resource="http://schema.org/description"/>
        <rdfs:domain>
            <owl:Class>
                <owl:intersectionOf rdf:parseType="Collection">
                    <rdf:Description rdf:about="http://linkedscience.org/teach/ns#Assignment"/>
                    <rdf:Description rdf:about="http://purl.org/he/syllabus/ontology#Assessment"/>
                    <rdf:Description rdf:about="http://purl.org/he/syllabus/ontology#Classroom"/>
                    <rdf:Description rdf:about="http://purl.org/he/syllabus/ontology#Help"/>
                    <rdf:Description rdf:about="http://purl.org/he/syllabus/ontology#Methodology"/>
                    <rdf:Description rdf:about="http://purl.org/he/syllabus/ontology#Policy"/>
                    <rdf:Description rdf:about="http://purl.org/he/syllabus/ontology#Syllabus"/>
                    <rdf:Description rdf:about="http://vivoweb.org/ontology/core#Course"/>
                </owl:intersectionOf>
            </owl:Class>
        </rdfs:domain>
        <rdfs:range rdf:resource="http://www.w3.org/2001/XMLSchema#string"/>
        <rdfs:comment>An account of the resource.</rdfs:comment>
        <rdfs:label>description</rdfs:label>
    </owl:DatatypeProperty>
    


    <!-- http://purl.org/dc/terms/hasVersion -->

    <owl:DatatypeProperty rdf:about="http://purl.org/dc/terms/hasVersion">
        <rdfs:domain rdf:resource="http://purl.org/he/syllabus/ontology#Syllabus"/>
        <rdfs:range rdf:resource="http://www.w3.org/2001/XMLSchema#string"/>
        <rdfs:comment> A related resource that is a version, edition, or adaptation of the described resource.</rdfs:comment>
        <rdfs:label>version</rdfs:label>
    </owl:DatatypeProperty>
    


    <!-- http://purl.org/dc/terms/title -->

    <owl:DatatypeProperty rdf:about="http://purl.org/dc/terms/title">
        <rdfs:domain rdf:resource="http://purl.org/he/syllabus/ontology#Syllabus"/>
        <rdfs:range rdf:resource="http://www.w3.org/2001/XMLSchema#string"/>
        <rdfs:comment>A name given to the resource.</rdfs:comment>
        <rdfs:label>title</rdfs:label>
    </owl:DatatypeProperty>
    


    <!-- http://purl.org/he/syllabus/ontology#bibliographicCitation -->

    <owl:DatatypeProperty rdf:about="http://purl.org/he/syllabus/ontology#bibliographicCitation">
        <rdfs:domain rdf:resource="dct:BibliographicResource"/>
        <rdfs:range rdf:resource="http://www.w3.org/2001/XMLSchema#string"/>
        <rdfs:comment>A bibliographic reference for the resource.</rdfs:comment>
        <rdfs:label>bibliographic citation</rdfs:label>
    </owl:DatatypeProperty>
    


    <!-- http://purl.org/he/syllabus/ontology#deadline -->

    <owl:DatatypeProperty rdf:about="http://purl.org/he/syllabus/ontology#deadline">
        <rdfs:domain>
            <owl:Class>
                <owl:intersectionOf rdf:parseType="Collection">
                    <rdf:Description rdf:about="http://linkedscience.org/teach/ns#Assignment"/>
                    <rdf:Description rdf:about="http://purl.org/he/syllabus/ontology#Assessment"/>
                </owl:intersectionOf>
            </owl:Class>
        </rdfs:domain>
        <rdfs:range rdf:resource="http://www.w3.org/2001/XMLSchema#dateTime"/>
        <rdfs:comment>Date the content expires and is no longer useful or available.</rdfs:comment>
        <rdfs:label>deadline</rdfs:label>
    </owl:DatatypeProperty>
    


    <!-- http://purl.org/he/syllabus/ontology#durationPerTerm -->

    <owl:DatatypeProperty rdf:about="http://purl.org/he/syllabus/ontology#durationPerTerm">
        <rdfs:domain rdf:resource="http://purl.org/he/syllabus/ontology#Workload"/>
        <rdfs:range rdf:resource="http://www.w3.org/2001/XMLSchema#nonNegativeInteger"/>
        <rdfs:comment>duration of workload per term</rdfs:comment>
        <rdfs:label>duration per term</rdfs:label>
    </owl:DatatypeProperty>
    


    <!-- http://purl.org/he/syllabus/ontology#durationPerWeek -->

    <owl:DatatypeProperty rdf:about="http://purl.org/he/syllabus/ontology#durationPerWeek">
        <rdfs:domain rdf:resource="http://purl.org/he/syllabus/ontology#Workload"/>
        <rdfs:range rdf:resource="http://www.w3.org/2001/XMLSchema#nonNegativeInteger"/>
        <rdfs:comment>duration of workload per week</rdfs:comment>
        <rdfs:label>duration per week</rdfs:label>
    </owl:DatatypeProperty>
    


    <!-- http://purl.org/he/syllabus/ontology#educationLevel -->

    <owl:DatatypeProperty rdf:about="http://purl.org/he/syllabus/ontology#educationLevel">
        <rdfs:domain rdf:resource="http://vivoweb.org/ontology/core#AcademicDegree"/>
        <rdfs:range rdf:resource="http://www.w3.org/2001/XMLSchema#string"/>
        <rdfs:comment>A class of entity, defined in terms of progression through an educational or training context, for which the described resource is intended</rdfs:comment>
        <rdfs:label>education level</rdfs:label>
    </owl:DatatypeProperty>
    


    <!-- http://purl.org/he/syllabus/ontology#number -->

    <owl:DatatypeProperty rdf:about="http://purl.org/he/syllabus/ontology#number">
        <rdfs:domain>
            <owl:Class>
                <owl:intersectionOf rdf:parseType="Collection">
                    <rdf:Description rdf:about="http://linkedscience.org/teach/ns#Assignment"/>
                    <rdf:Description rdf:about="http://purl.org/he/syllabus/ontology#Assessment"/>
                    <rdf:Description rdf:about="http://purl.org/he/syllabus/ontology#Classroom"/>
                </owl:intersectionOf>
            </owl:Class>
        </rdfs:domain>
        <rdfs:range rdf:resource="http://www.w3.org/2001/XMLSchema#string"/>
        <rdfs:comment>The number of a class or activity.</rdfs:comment>
        <rdfs:label>number</rdfs:label>
    </owl:DatatypeProperty>
    


    <!-- http://purl.org/he/syllabus/ontology#office -->

    <owl:DatatypeProperty rdf:about="http://purl.org/he/syllabus/ontology#office">
        <rdfs:domain rdf:resource="http://purl.org/he/syllabus/ontology#Instructor"/>
        <rdfs:range rdf:resource="http://www.w3.org/2001/XMLSchema#string"/>
        <rdfs:comment>Office of the teacher</rdfs:comment>
        <rdfs:label>office</rdfs:label>
    </owl:DatatypeProperty>
    


    <!-- http://purl.org/he/syllabus/ontology#order -->

    <owl:DatatypeProperty rdf:about="http://purl.org/he/syllabus/ontology#order">
        <rdfs:domain rdf:resource="http://purl.org/he/syllabus/ontology#Topic"/>
        <rdfs:range rdf:resource="http://www.w3.org/2001/XMLSchema#string"/>
        <rdfs:comment>The sequence in which the study topics are arranged.</rdfs:comment>
        <rdfs:label>order</rdfs:label>
    </owl:DatatypeProperty>
    


    <!-- http://purl.org/he/syllabus/ontology#requirement -->

    <owl:DatatypeProperty rdf:about="http://purl.org/he/syllabus/ontology#requirement">
        <rdfs:domain rdf:resource="http://purl.org/he/syllabus/ontology#Syllabus"/>
        <rdfs:range rdf:resource="http://www.w3.org/2001/XMLSchema#string"/>
        <rdfs:comment>Requirements for taking the Course. May be completion of another Course or a textual description like &quot;permission of instructor&quot;. Requirements may be a pre-requisite competency, referenced using AlignmentObject.</rdfs:comment>
        <rdfs:label>requirement</rdfs:label>
    </owl:DatatypeProperty>
    


    <!-- http://purl.org/he/syllabus/ontology#resume -->

    <owl:DatatypeProperty rdf:about="http://purl.org/he/syllabus/ontology#resume">
        <rdfs:domain rdf:resource="http://purl.org/he/syllabus/ontology#Instructor"/>
        <rdfs:range rdf:resource="http://www.w3.org/2001/XMLSchema#string"/>
        <rdfs:comment>Short written description of the teacher experience.</rdfs:comment>
        <rdfs:label>resume</rdfs:label>
    </owl:DatatypeProperty>
    


    <!-- http://purl.org/he/syllabus/ontology#score -->

    <owl:DatatypeProperty rdf:about="http://purl.org/he/syllabus/ontology#score">
        <rdfs:domain>
            <owl:Class>
                <owl:intersectionOf rdf:parseType="Collection">
                    <rdf:Description rdf:about="http://linkedscience.org/teach/ns#Assignment"/>
                    <rdf:Description rdf:about="http://purl.org/he/syllabus/ontology#Assessment"/>
                </owl:intersectionOf>
            </owl:Class>
        </rdfs:domain>
        <rdfs:range rdf:resource="http://www.w3.org/2001/XMLSchema#string"/>
        <rdfs:comment>The number of points obtained in an evaluation.</rdfs:comment>
        <rdfs:label>score</rdfs:label>
    </owl:DatatypeProperty>
    


    <!-- http://purl.org/he/syllabus/ontology#studyStrategy -->

    <owl:DatatypeProperty rdf:about="http://purl.org/he/syllabus/ontology#studyStrategy">
        <rdfs:domain rdf:resource="http://purl.org/he/syllabus/ontology#Methodology"/>
        <rdfs:range rdf:resource="http://www.w3.org/2001/XMLSchema#string"/>
        <rdfs:comment>Study tips or strategies to improve your studies.</rdfs:comment>
        <rdfs:label>study strategy</rdfs:label>
    </owl:DatatypeProperty>
    


    <!-- http://purl.org/he/syllabus/ontology#type -->

    <owl:DatatypeProperty rdf:about="http://purl.org/he/syllabus/ontology#type">
        <rdfs:domain>
            <owl:Class>
                <owl:intersectionOf rdf:parseType="Collection">
                    <rdf:Description rdf:about="dct:BibliographicResource"/>
                    <rdf:Description rdf:about="http://linkedscience.org/teach/ns#Assignment"/>
                    <rdf:Description rdf:about="http://purl.org/he/syllabus/ontology#Assessment"/>
                    <rdf:Description rdf:about="http://purl.org/he/syllabus/ontology#Classroom"/>
                    <rdf:Description rdf:about="http://purl.org/he/syllabus/ontology#Instructor"/>
                    <rdf:Description rdf:about="http://purl.org/he/syllabus/ontology#Topic"/>
                    <rdf:Description rdf:about="http://vivoweb.org/ontology/core#Course"/>
                </owl:intersectionOf>
            </owl:Class>
        </rdfs:domain>
        <rdfs:range rdf:resource="http://www.w3.org/2001/XMLSchema#string"/>
        <rdfs:comment>Category or type of something.</rdfs:comment>
        <rdfs:label>type</rdfs:label>
    </owl:DatatypeProperty>
    


    <!-- http://purl.org/he/syllabus/ontology#unitPerTerm -->

    <owl:DatatypeProperty rdf:about="http://purl.org/he/syllabus/ontology#unitPerTerm">
        <rdfs:domain rdf:resource="http://purl.org/he/syllabus/ontology#Workload"/>
        <rdfs:range rdf:resource="http://www.w3.org/2001/XMLSchema#string"/>
        <rdfs:comment>unit to measure workload by term</rdfs:comment>
        <rdfs:label>unit per term</rdfs:label>
    </owl:DatatypeProperty>
    


    <!-- http://purl.org/he/syllabus/ontology#unitPerWeek -->

    <owl:DatatypeProperty rdf:about="http://purl.org/he/syllabus/ontology#unitPerWeek">
        <rdfs:domain rdf:resource="http://purl.org/he/syllabus/ontology#Workload"/>
        <rdfs:range rdf:resource="http://www.w3.org/2001/XMLSchema#string"/>
        <rdfs:comment>unit to measure workload by week</rdfs:comment>
        <rdfs:label>unit per week</rdfs:label>
    </owl:DatatypeProperty>
    


    <!-- http://purl.org/he/syllabus/ontology#weight -->

    <owl:DatatypeProperty rdf:about="http://purl.org/he/syllabus/ontology#weight">
        <rdfs:domain>
            <owl:Class>
                <owl:intersectionOf rdf:parseType="Collection">
                    <rdf:Description rdf:about="http://linkedscience.org/teach/ns#Assignment"/>
                    <rdf:Description rdf:about="http://purl.org/he/syllabus/ontology#Assessment"/>
                </owl:intersectionOf>
            </owl:Class>
        </rdfs:domain>
        <rdfs:range rdf:resource="http://www.w3.org/2001/XMLSchema#string"/>
        <rdfs:comment>weight of the assignment</rdfs:comment>
        <rdfs:label>weight</rdfs:label>
    </owl:DatatypeProperty>
    


    <!-- http://purl.org/vocab/aiiso/schema#code -->

    <owl:DatatypeProperty rdf:about="http://purl.org/vocab/aiiso/schema#code">
        <owl:equivalentProperty rdf:resource="http://schema.org/courseCode"/>
        <rdfs:domain rdf:resource="http://schema.org/Course"/>
        <rdfs:range rdf:resource="http://www.w3.org/2001/XMLSchema#string"/>
        <rdfs:comment>A person assigned to instruct or provide instructional assistance for the CourseInstance.</rdfs:comment>
        <rdfs:label>code</rdfs:label>
    </owl:DatatypeProperty>
    


    <!-- http://schema.org/courseCode -->

    <owl:DatatypeProperty rdf:about="http://schema.org/courseCode">
        <rdfs:domain rdf:resource="http://schema.org/Course"/>
        <rdfs:range rdf:resource="http://www.w3.org/2001/XMLSchema#string"/>
        <rdfs:comment>The identifier for the Course used by the course provider.</rdfs:comment>
        <rdfs:label>code</rdfs:label>
    </owl:DatatypeProperty>
    


    <!-- http://schema.org/courseMode -->

    <owl:DatatypeProperty rdf:about="http://schema.org/courseMode">
        <rdfs:subPropertyOf rdf:resource="http://www.w3.org/2002/07/owl#topDataProperty"/>
        <rdfs:domain rdf:resource="http://schema.org/CourseInstance"/>
        <rdfs:range rdf:resource="http://www.w3.org/2001/XMLSchema#string"/>
        <rdfs:comment>The medium or means of delivery of the course instance or the mode of study, either as a text label (e.g. &quot;online&quot;, &quot;onsite&quot; or &quot;blended&quot;; &quot;synchronous&quot; or &quot;asynchronous&quot;; &quot;full-time&quot; or &quot;part-time&quot;) or as a URL reference to a term from a controlled vocabulary.</rdfs:comment>
        <rdfs:label>course mode</rdfs:label>
    </owl:DatatypeProperty>
    


    <!-- http://schema.org/description -->

    <owl:DatatypeProperty rdf:about="http://schema.org/description">
        <rdfs:domain>
            <owl:Class>
                <owl:intersectionOf rdf:parseType="Collection">
                    <rdf:Description rdf:about="http://linkedscience.org/teach/ns#Assignment"/>
                    <rdf:Description rdf:about="http://purl.org/he/syllabus/ontology#Assessment"/>
                    <rdf:Description rdf:about="http://purl.org/he/syllabus/ontology#Classroom"/>
                    <rdf:Description rdf:about="http://purl.org/he/syllabus/ontology#Help"/>
                    <rdf:Description rdf:about="http://purl.org/he/syllabus/ontology#Methodology"/>
                    <rdf:Description rdf:about="http://purl.org/he/syllabus/ontology#Policy"/>
                    <rdf:Description rdf:about="http://purl.org/he/syllabus/ontology#Syllabus"/>
                    <rdf:Description rdf:about="http://vivoweb.org/ontology/core#Course"/>
                </owl:intersectionOf>
            </owl:Class>
        </rdfs:domain>
        <rdfs:range rdf:resource="http://www.w3.org/2001/XMLSchema#string"/>
        <rdfs:comment>A description of the item.</rdfs:comment>
        <rdfs:label>description</rdfs:label>
    </owl:DatatypeProperty>
    


    <!-- http://schema.org/email -->

    <owl:DatatypeProperty rdf:about="http://schema.org/email">
        <rdfs:domain rdf:resource="http://schema.org/Agent"/>
        <rdfs:range rdf:resource="http://www.w3.org/2001/XMLSchema#string"/>
        <rdfs:comment>Email address.</rdfs:comment>
        <rdfs:label>email</rdfs:label>
    </owl:DatatypeProperty>
    


    <!-- http://schema.org/name -->

    <owl:DatatypeProperty rdf:about="http://schema.org/name">
        <owl:equivalentProperty rdf:resource="http://xmlns.com/foaf/0.1/name"/>
        <rdfs:domain>
            <owl:Class>
                <owl:intersectionOf rdf:parseType="Collection">
                    <rdf:Description rdf:about="http://schema.org/Agent"/>
                    <rdf:Description rdf:about="http://vivoweb.org/ontology/core#Course"/>
                </owl:intersectionOf>
            </owl:Class>
        </rdfs:domain>
        <rdfs:range rdf:resource="http://www.w3.org/2001/XMLSchema#string"/>
        <rdfs:comment>The name of the item.</rdfs:comment>
        <rdfs:label>name</rdfs:label>
    </owl:DatatypeProperty>
    


    <!-- http://schema.org/telephone -->

    <owl:DatatypeProperty rdf:about="http://schema.org/telephone">
        <rdfs:domain rdf:resource="http://schema.org/Agent"/>
        <rdfs:range rdf:resource="http://www.w3.org/2001/XMLSchema#string"/>
        <rdfs:comment>The telephone number.</rdfs:comment>
        <rdfs:label>telephone</rdfs:label>
    </owl:DatatypeProperty>
    


    <!-- http://schema.org/url -->

    <owl:DatatypeProperty rdf:about="http://schema.org/url">
        <rdfs:domain>
            <owl:Class>
                <owl:intersectionOf rdf:parseType="Collection">
                    <rdf:Description rdf:about="http://purl.org/he/syllabus/ontology#Syllabus"/>
                    <rdf:Description rdf:about="http://xmlns.com/foaf/0.1/Agent"/>
                </owl:intersectionOf>
            </owl:Class>
        </rdfs:domain>
        <rdfs:range rdf:resource="http://www.w3.org/2001/XMLSchema#string"/>
        <rdfs:comment>URL of the resource</rdfs:comment>
        <rdfs:label>url</rdfs:label>
    </owl:DatatypeProperty>
    


    <!-- http://vivoweb.org/ontology/core#courseCredits -->

    <owl:DatatypeProperty rdf:about="http://vivoweb.org/ontology/core#courseCredits">
        <rdfs:domain rdf:resource="http://schema.org/Course"/>
        <rdfs:range rdf:resource="http://www.w3.org/2001/XMLSchema#string"/>
        <rdfs:comment>Number of credits assigned a course by an learning institution.</rdfs:comment>
        <rdfs:label>course credits</rdfs:label>
    </owl:DatatypeProperty>
    


    <!-- http://www.ontologydesignpatterns.org/cp/owl/timeinterval.owl#hasIntervalDate -->

    <owl:DatatypeProperty rdf:about="http://www.ontologydesignpatterns.org/cp/owl/timeinterval.owl#hasIntervalDate">
        <rdfs:domain rdf:resource="http://www.ontologydesignpatterns.org/cp/owl/timeinterval.owl#TimeInterval"/>
        <rdfs:range rdf:resource="http://www.w3.org/2001/XMLSchema#dateTime"/>
        <rdfs:comment>A datatype property that encodes values from xsd:date for a time interval; a same time interval can have more than one xsd:date value: begin date, end date, date at which the interval holds, as well as dates expressed in different formats: xsd:gYear, xsd:dateTime, etc.</rdfs:comment>
        <rdfs:label>has interval date</rdfs:label>
    </owl:DatatypeProperty>
    


    <!-- http://www.ontologydesignpatterns.org/cp/owl/timeinterval.owl#hasIntervalEndDate -->

    <owl:DatatypeProperty rdf:about="http://www.ontologydesignpatterns.org/cp/owl/timeinterval.owl#hasIntervalEndDate">
        <rdfs:domain rdf:resource="http://www.ontologydesignpatterns.org/cp/owl/timeinterval.owl#TimeInterval"/>
        <rdfs:range rdf:resource="http://www.w3.org/2001/XMLSchema#dateTime"/>
        <rdfs:comment>The end date of a time interval.</rdfs:comment>
        <rdfs:label>end date</rdfs:label>
    </owl:DatatypeProperty>
    


    <!-- http://www.ontologydesignpatterns.org/cp/owl/timeinterval.owl#hasIntervalStartDate -->

    <owl:DatatypeProperty rdf:about="http://www.ontologydesignpatterns.org/cp/owl/timeinterval.owl#hasIntervalStartDate">
        <rdfs:domain rdf:resource="http://www.ontologydesignpatterns.org/cp/owl/timeinterval.owl#TimeInterval"/>
        <rdfs:range rdf:resource="http://www.w3.org/2001/XMLSchema#dateTime"/>
        <rdfs:comment>The start date of a time interval.</rdfs:comment>
        <rdfs:label>start date</rdfs:label>
    </owl:DatatypeProperty>
    


    <!-- http://xmlns.com/foaf/0.1/name -->

    <owl:DatatypeProperty rdf:about="http://xmlns.com/foaf/0.1/name">
        <rdfs:domain>
            <owl:Class>
                <owl:intersectionOf rdf:parseType="Collection">
                    <rdf:Description rdf:about="http://schema.org/Agent"/>
                    <rdf:Description rdf:about="http://vivoweb.org/ontology/core#Course"/>
                </owl:intersectionOf>
            </owl:Class>
        </rdfs:domain>
        <rdfs:range rdf:resource="http://www.w3.org/2001/XMLSchema#string"/>
        <rdfs:comment>The name of something is a simple textual string.</rdfs:comment>
        <rdfs:label>name</rdfs:label>
    </owl:DatatypeProperty>
    


    <!-- 
    ///////////////////////////////////////////////////////////////////////////////////////
    //
    // Classes
    //
    ///////////////////////////////////////////////////////////////////////////////////////
     -->

    


    <!-- dct:BibliographicResource -->

    <owl:Class rdf:about="dct:BibliographicResource">
        <rdfs:comment>A book, article, or other documentary resource.</rdfs:comment>
        <rdfs:label>Bibliographic Resource</rdfs:label>
        <rdfs:label>Learning Resource</rdfs:label>
    </owl:Class>
    


    <!-- http://linkedscience.org/teach/ns#Assignment -->

    <owl:Class rdf:about="http://linkedscience.org/teach/ns#Assignment">
        <rdfs:comment>Assignment of a course, for example an exercise.</rdfs:comment>
        <rdfs:label>Assignment</rdfs:label>
    </owl:Class>
    


    <!-- http://linkedscience.org/teach/ns#Course -->

    <owl:Class rdf:about="http://linkedscience.org/teach/ns#Course">
        <owl:equivalentClass rdf:resource="http://schema.org/Course"/>
        <rdfs:comment>Course is where students are supposed to learn something.</rdfs:comment>
        <rdfs:label>Course</rdfs:label>
    </owl:Class>
    


    <!-- http://linkedscience.org/teach/ns#Teacher -->

    <owl:Class rdf:about="http://linkedscience.org/teach/ns#Teacher">
        <owl:equivalentClass rdf:resource="http://purl.org/he/syllabus/ontology#Instructor"/>
        <rdfs:comment>Teacher of the course.</rdfs:comment>
        <rdfs:label>Professor</rdfs:label>
        <rdfs:label>Teacher</rdfs:label>
    </owl:Class>
    


    <!-- http://purl.org/dc/terms/LinguisticSystem -->

    <owl:Class rdf:about="http://purl.org/dc/terms/LinguisticSystem">
        <rdfs:comment>A system of signs, symbols, sounds, gestures, or rules used in communication.</rdfs:comment>
        <rdfs:label>Language</rdfs:label>
        <rdfs:label>Lingüistic System</rdfs:label>
    </owl:Class>
    


    <!-- http://purl.org/he/syllabus/ontology#Accessibility -->

    <owl:Class rdf:about="http://purl.org/he/syllabus/ontology#Accessibility">
        <rdfs:subClassOf rdf:resource="http://purl.org/he/syllabus/ontology#Policy"/>
        <rdfs:comment>Policy to meet the requirements for class adaptation for students with disabilities.</rdfs:comment>
        <rdfs:label>Accessibility</rdfs:label>
    </owl:Class>
    


    <!-- http://purl.org/he/syllabus/ontology#Assessment -->

    <owl:Class rdf:about="http://purl.org/he/syllabus/ontology#Assessment">
        <rdfs:comment>Refers to the wide variety of methods or tools that educators use to evaluate, measure, and document the academic readiness, learning progress, skill acquisition, or educational needs of students.</rdfs:comment>
        <rdfs:label>Assessment</rdfs:label>
    </owl:Class>
    


    <!-- http://purl.org/he/syllabus/ontology#Attendance -->

    <owl:Class rdf:about="http://purl.org/he/syllabus/ontology#Attendance">
        <rdfs:subClassOf rdf:resource="http://purl.org/he/syllabus/ontology#Policy"/>
        <rdfs:comment>Defines absences and tardiness, includes rules for attendance, and lays out disciplinary actions.</rdfs:comment>
        <rdfs:label>Attendance Policy</rdfs:label>
    </owl:Class>
    


    <!-- http://purl.org/he/syllabus/ontology#Classroom -->

    <owl:Class rdf:about="http://purl.org/he/syllabus/ontology#Classroom">
        <rdfs:comment>A room in an educational intitution where groups of students are taught</rdfs:comment>
        <rdfs:label>Classroom</rdfs:label>
    </owl:Class>
    


    <!-- http://purl.org/he/syllabus/ontology#Competence -->

    <owl:Class rdf:about="http://purl.org/he/syllabus/ontology#Competence">
        <owl:equivalentClass rdf:resource="http://www.teste/ontologies/IEEE_RCD_Impl.owlCompetence"/>
        <rdfs:subClassOf rdf:resource="http://purl.org/he/syllabus/ontology#GoalStatement"/>
        <rdfs:comment>A very specific statement that describes exactly what a student will be able to do in some measurable way. There may be more than one measurable outcome defined for a given competency.</rdfs:comment>
        <rdfs:label>Competence</rdfs:label>
        <rdfs:label>Competency</rdfs:label>
    </owl:Class>
    


    <!-- http://purl.org/he/syllabus/ontology#Content -->

    <owl:Class rdf:about="http://purl.org/he/syllabus/ontology#Content">
        <rdfs:subClassOf rdf:resource="http://www.w3.org/2004/02/skos/core#Collection"/>
        <rdfs:comment>A list of subunits of the resource.</rdfs:comment>
        <rdfs:label>Content</rdfs:label>
    </owl:Class>
    


    <!-- http://purl.org/he/syllabus/ontology#DropOut -->

    <owl:Class rdf:about="http://purl.org/he/syllabus/ontology#DropOut">
        <rdfs:subClassOf rdf:resource="http://purl.org/he/syllabus/ontology#Policy"/>
        <rdfs:comment>Defines the actions by which a student may be removed from the course</rdfs:comment>
        <rdfs:label>Drop out policy</rdfs:label>
    </owl:Class>
    


    <!-- http://purl.org/he/syllabus/ontology#GoalStatement -->

    <owl:Class rdf:about="http://purl.org/he/syllabus/ontology#GoalStatement">
        <rdfs:comment>The goal statement is one of the most important parts of the definition syllabus. With clearly and concisely stated goals, the rest of the planning process falls naturally into place.</rdfs:comment>
        <rdfs:label>Goal Statement</rdfs:label>
    </owl:Class>
    


    <!-- http://purl.org/he/syllabus/ontology#Help -->

    <owl:Class rdf:about="http://purl.org/he/syllabus/ontology#Help">
        <rdfs:comment>Information or advice given to reach success in a course</rdfs:comment>
        <rdfs:label>Help</rdfs:label>
    </owl:Class>
    


    <!-- http://purl.org/he/syllabus/ontology#Instructor -->

    <owl:Class rdf:about="http://purl.org/he/syllabus/ontology#Instructor">
        <rdfs:subClassOf rdf:resource="http://schema.org/Person"/>
        <rdfs:comment>A person assigned to instruct or provide instructional assistance for the CourseInstance.</rdfs:comment>
        <rdfs:label>Instructor</rdfs:label>
        <rdfs:label>Professor</rdfs:label>
        <rdfs:label>Teacher</rdfs:label>
    </owl:Class>
    


    <!-- http://purl.org/he/syllabus/ontology#LearningObjective -->

    <owl:Class rdf:about="http://purl.org/he/syllabus/ontology#LearningObjective">
        <rdfs:subClassOf rdf:resource="http://purl.org/he/syllabus/ontology#GoalStatement"/>
        <rdfs:comment>Learning objectives are statements that define the expected goal of a curriculum, course, lesson or activity interms of demonstrable skills or knowledge that will be acquired by a student as a result of instruction.</rdfs:comment>
        <rdfs:label>Learning objective</rdfs:label>
    </owl:Class>
    


    <!-- http://purl.org/he/syllabus/ontology#LearningOutcome -->

    <owl:Class rdf:about="http://purl.org/he/syllabus/ontology#LearningOutcome">
        <rdfs:subClassOf rdf:resource="http://purl.org/he/syllabus/ontology#GoalStatement"/>
        <rdfs:comment>Learning outcomes are statements that describe significant and essential learning that learners have achieved, and can reliably demonstrate at the end of a course or program. In other words, learning outcomes identify what the learner will know and be able to do by the end of a course or program.</rdfs:comment>
        <rdfs:label>Learning outcome</rdfs:label>
    </owl:Class>
    


    <!-- http://purl.org/he/syllabus/ontology#Methodology -->

    <owl:Class rdf:about="http://purl.org/he/syllabus/ontology#Methodology">
        <rdfs:comment>A system of ways of doing, teaching, or studying something.</rdfs:comment>
        <rdfs:label>Methodology</rdfs:label>
    </owl:Class>
    


    <!-- http://purl.org/he/syllabus/ontology#Policy -->

    <owl:Class rdf:about="http://purl.org/he/syllabus/ontology#Policy">
        <rdfs:comment>Education policy are the principles and government policy-making in the educational sphere.</rdfs:comment>
        <rdfs:label>Educational Policy</rdfs:label>
    </owl:Class>
    


    <!-- http://purl.org/he/syllabus/ontology#Qualification -->

    <owl:Class rdf:about="http://purl.org/he/syllabus/ontology#Qualification">
        <rdfs:subClassOf rdf:resource="http://purl.org/he/syllabus/ontology#Policy"/>
        <rdfs:comment>The rules that determine a qualification.</rdfs:comment>
        <rdfs:label>Qualification Policy</rdfs:label>
    </owl:Class>
    


    <!-- http://purl.org/he/syllabus/ontology#Reviewer -->

    <owl:Class rdf:about="http://purl.org/he/syllabus/ontology#Reviewer">
        <rdfs:subClassOf rdf:resource="http://purl.org/spar/pro/Role"/>
        <rdfs:comment>The person who monitors, directs and approves the activities carried out by a group of people.</rdfs:comment>
        <rdfs:label>Entity that approves a Syllabus</rdfs:label>
    </owl:Class>
    


    <!-- http://purl.org/he/syllabus/ontology#Schedule -->

    <owl:Class rdf:about="http://purl.org/he/syllabus/ontology#Schedule">
        <rdfs:comment>Schedule of the class. It apply for tutoring, classes, laboratory, etc.</rdfs:comment>
        <rdfs:label>Schedule</rdfs:label>
    </owl:Class>
    


    <!-- http://purl.org/he/syllabus/ontology#Syllabus -->

    <owl:Class rdf:about="http://purl.org/he/syllabus/ontology#Syllabus">
        <rdfs:subClassOf rdf:resource="http://purl.org/vocab/frbr/core#Work"/>
        <rdfs:comment>A syllabus is a document that outlines everything that will be covered in a course</rdfs:comment>
        <rdfs:label>Syllabus</rdfs:label>
    </owl:Class>
    


    <!-- http://purl.org/he/syllabus/ontology#Topic -->

    <owl:Class rdf:about="http://purl.org/he/syllabus/ontology#Topic">
        <rdfs:subClassOf rdf:resource="http://www.w3.org/2004/02/skos/core#Concept"/>
        <rdfs:comment>The topic or the subject of the course.</rdfs:comment>
        <rdfs:label>Subject</rdfs:label>
        <rdfs:label>Topic</rdfs:label>
    </owl:Class>
    


    <!-- http://purl.org/he/syllabus/ontology#Workload -->

    <owl:Class rdf:about="http://purl.org/he/syllabus/ontology#Workload">
        <rdfs:comment>The amount of work or of working time expected or assigned to do an activity.</rdfs:comment>
        <rdfs:label>WorkLoad</rdfs:label>
    </owl:Class>
    


    <!-- http://purl.org/spar/pro/Role -->

    <owl:Class rdf:about="http://purl.org/spar/pro/Role">
        <rdfs:comment>A role an agent may have. Individual members of this class or its sub-classes are used to specify particular roles.</rdfs:comment>
        <rdfs:label>Role</rdfs:label>
    </owl:Class>
    


    <!-- http://purl.org/spar/pro/RoleInTime -->

    <owl:Class rdf:about="http://purl.org/spar/pro/RoleInTime">
        <rdfs:comment>A particular situation that describe a role an agent may have, that can be restricted to a particular time interval.</rdfs:comment>
        <rdfs:label>Role in Time</rdfs:label>
    </owl:Class>
    


    <!-- http://purl.org/vocab/aiiso/schema#Course -->

    <owl:Class rdf:about="http://purl.org/vocab/aiiso/schema#Course">
        <owl:equivalentClass rdf:resource="http://schema.org/Course"/>
        <rdfs:comment>A course is a KnowledgeGrouping that represents a cohesive collection of educational material referred to by the owning organization as a course.</rdfs:comment>
        <rdfs:label>Course</rdfs:label>
    </owl:Class>
    


    <!-- http://purl.org/vocab/aiiso/schema#Department -->

    <owl:Class rdf:about="http://purl.org/vocab/aiiso/schema#Department">
        <rdfs:subClassOf rdf:resource="http://schema.org/Organization"/>
        <rdfs:comment>A Department is a group of people recognised by an organization as forming a cohesive group referred to by the organization as a department.</rdfs:comment>
        <rdfs:label>Department</rdfs:label>
    </owl:Class>
    


    <!-- http://purl.org/vocab/aiiso/schema#Faculty -->

    <owl:Class rdf:about="http://purl.org/vocab/aiiso/schema#Faculty">
        <rdfs:subClassOf rdf:resource="http://schema.org/Organization"/>
        <rdfs:comment></rdfs:comment>
        <rdfs:comment>A Faculty is a group of people recognised by an organization as forming a cohesive group referred to by the organization as a faculty.</rdfs:comment>
        <rdfs:label>Faculty</rdfs:label>
    </owl:Class>
    


    <!-- http://purl.org/vocab/aiiso/schema#KnowledgeGrouping -->

    <owl:Class rdf:about="http://purl.org/vocab/aiiso/schema#KnowledgeGrouping">
        <rdfs:comment>A KnowledgeGrouping represents a collection of resources, learning objectives, timetables, and other materials.</rdfs:comment>
        <rdfs:label>Knowledge Grouping</rdfs:label>
    </owl:Class>
    


    <!-- http://purl.org/vocab/aiiso/schema#School -->

    <owl:Class rdf:about="http://purl.org/vocab/aiiso/schema#School">
        <rdfs:subClassOf rdf:resource="http://schema.org/Organization"/>
        <rdfs:comment>A School is a group of people recognised by an organization as forming a cohesive group referred to by the organization as a school.</rdfs:comment>
        <rdfs:label>School</rdfs:label>
    </owl:Class>
    


    <!-- http://purl.org/vocab/frbr/core#Expression -->

    <owl:Class rdf:about="http://purl.org/vocab/frbr/core#Expression">
        <rdfs:comment>The intellectual or artistic realization of a work in the form of alpha-numeric, musical, or choreographic notation, sound, image, object, movement, etc., or any combination of such forms.</rdfs:comment>
        <rdfs:label>Expression</rdfs:label>
    </owl:Class>
    


    <!-- http://purl.org/vocab/frbr/core#Manifestation -->

    <owl:Class rdf:about="http://purl.org/vocab/frbr/core#Manifestation">
        <rdfs:comment>The physical embodiment of an expression of a work.</rdfs:comment>
        <rdfs:label>Manifestation</rdfs:label>
    </owl:Class>
    


    <!-- http://purl.org/vocab/frbr/core#Work -->

    <owl:Class rdf:about="http://purl.org/vocab/frbr/core#Work">
        <rdfs:comment>A distinct intellectual or artistic creation.</rdfs:comment>
        <rdfs:label>Work</rdfs:label>
    </owl:Class>
    


    <!-- http://schema.org/Agent -->

    <owl:Class rdf:about="http://schema.org/Agent">
        <owl:equivalentClass rdf:resource="http://xmlns.com/foaf/0.1/Agent"/>
        <rdfs:comment>The direct performer or driver of the action.</rdfs:comment>
        <rdfs:label>Agent</rdfs:label>
    </owl:Class>
    


    <!-- http://schema.org/Audience -->

    <owl:Class rdf:about="http://schema.org/Audience">
        <rdfs:comment>Intended audience for an item, i.e. the group for whom the item was created.</rdfs:comment>
        <rdfs:label>Audience</rdfs:label>
    </owl:Class>
    


    <!-- http://schema.org/Course -->

    <owl:Class rdf:about="http://schema.org/Course">
        <owl:equivalentClass rdf:resource="http://vivoweb.org/ontology/core#Course"/>
        <rdfs:comment>A description of an educational course which may be offered as distinct instances at which take place at different times or take place at different locations, or be offered through different media or modes of study. An educational course is a sequence of one or more educational events and/or creative works which aims to build knowledge, competence or ability of learners.</rdfs:comment>
        <rdfs:label>Course</rdfs:label>
    </owl:Class>
    


    <!-- http://schema.org/CourseInstance -->

    <owl:Class rdf:about="http://schema.org/CourseInstance">
        <rdfs:comment>An instance of a Course which is distinct from other instances because it is offered at a different time or location or through different media or modes of study or to a specific section of students.</rdfs:comment>
        <rdfs:label>Course instance</rdfs:label>
    </owl:Class>
    


    <!-- http://schema.org/EducationalOrganization -->

    <owl:Class rdf:about="http://schema.org/EducationalOrganization">
        <rdfs:subClassOf rdf:resource="http://schema.org/Organization"/>
        <rdfs:comment>An educational organization.</rdfs:comment>
        <rdfs:label>Educational Organization</rdfs:label>
    </owl:Class>
    


    <!-- http://schema.org/Organization -->

    <owl:Class rdf:about="http://schema.org/Organization">
        <rdfs:subClassOf rdf:resource="http://schema.org/Agent"/>
        <rdfs:subClassOf rdf:resource="http://xmlns.com/foaf/0.1/Agent"/>
        <owl:disjointWith rdf:resource="http://xmlns.com/foaf/0.1/Person"/>
        <rdfs:comment>An organization such as a school.</rdfs:comment>
        <rdfs:comment>The Organization class represents a kind of Agent corresponding to social instititutions such as companies, societies etc.</rdfs:comment>
        <rdfs:label>Organization</rdfs:label>
    </owl:Class>
    


    <!-- http://schema.org/Person -->

    <owl:Class rdf:about="http://schema.org/Person">
        <owl:equivalentClass rdf:resource="http://xmlns.com/foaf/0.1/Person"/>
        <rdfs:subClassOf rdf:resource="http://schema.org/Agent"/>
        <rdfs:comment>A person (alive, dead, undead, of fictional).</rdfs:comment>
        <rdfs:label>Person</rdfs:label>
    </owl:Class>
    


    <!-- http://vivoweb.org/ontology/core#AcademicDegree -->

    <owl:Class rdf:about="http://vivoweb.org/ontology/core#AcademicDegree">
        <rdfs:comment>An academic degree at any level, both as reported by individuals for employment and as offered by academic degree programs.</rdfs:comment>
        <rdfs:label>Academic Degree</rdfs:label>
    </owl:Class>
    


    <!-- http://vivoweb.org/ontology/core#AcademicTerm -->

    <owl:Class rdf:about="http://vivoweb.org/ontology/core#AcademicTerm">
        <rdfs:comment>An explicit individual academic term, quarter, or semester rather than the generic fall, spring or summer semester.</rdfs:comment>
        <rdfs:label>Academic Term</rdfs:label>
    </owl:Class>
    


    <!-- http://vivoweb.org/ontology/core#AcademicYear -->

    <owl:Class rdf:about="http://vivoweb.org/ontology/core#AcademicYear">
        <rdfs:comment>An explicit individual period considered by an academic institution to be its primary academic cycle.</rdfs:comment>
        <rdfs:label>Academic Year</rdfs:label>
    </owl:Class>
    


    <!-- http://vivoweb.org/ontology/core#Course -->

    <owl:Class rdf:about="http://vivoweb.org/ontology/core#Course">
        <rdfs:comment>A course as taught in one time period by one or more instructors, normally but not always for credit.</rdfs:comment>
        <rdfs:label>Course</rdfs:label>
    </owl:Class>
    


    <!-- http://www.fonte-project.net/ontologies/SICRA.owlTaxonomiaBloom -->

    <owl:Class rdf:about="http://www.fonte-project.net/ontologies/SICRA.owlTaxonomiaBloom">
        <rdfs:comment>Bloom’s Taxonomy is a classification of the different objectives and skills that educators set for their students (learning objectives).</rdfs:comment>
        <rdfs:label>Bloom taxonomy</rdfs:label>
    </owl:Class>
    


    <!-- http://www.ontologydesignpatterns.org/cp/owl/timeinterval.owl#TimeInterval -->

    <owl:Class rdf:about="http://www.ontologydesignpatterns.org/cp/owl/timeinterval.owl#TimeInterval">
        <rdfs:comment>To represent time intervals.</rdfs:comment>
        <rdfs:label>Time Interval</rdfs:label>
    </owl:Class>
    


    <!-- http://www.teste/ontologies/IEEE_RCD_Impl.owlCompetence -->

    <owl:Class rdf:about="http://www.teste/ontologies/IEEE_RCD_Impl.owlCompetence">
        <rdfs:comment xml:lang="pt">Corresponde ao conceito &quot;Reusable Competency Definition&quot; da norma IEEE 1484.20.1</rdfs:comment>
        <rdfs:label>Competence</rdfs:label>
    </owl:Class>
    


    <!-- http://www.w3.org/2004/02/skos/core#Collection -->

    <owl:Class rdf:about="http://www.w3.org/2004/02/skos/core#Collection">
        <rdfs:comment>Collections are labeled and/or ordered groups of SKOS concepts.</rdfs:comment>
        <rdfs:label>Collection</rdfs:label>
    </owl:Class>
    


    <!-- http://www.w3.org/2004/02/skos/core#Concept -->

    <owl:Class rdf:about="http://www.w3.org/2004/02/skos/core#Concept">
        <rdfs:comment>A SKOS concept can be viewed as an idea or notion; a unit of thought.</rdfs:comment>
        <rdfs:label>Concept</rdfs:label>
    </owl:Class>
    


    <!-- http://xmlns.com/foaf/0.1/Agent -->

    <owl:Class rdf:about="http://xmlns.com/foaf/0.1/Agent">
        <rdfs:comment>An agent (eg. person, group, software or physical artifact). </rdfs:comment>
        <rdfs:label>Agent</rdfs:label>
    </owl:Class>
    


    <!-- http://xmlns.com/foaf/0.1/Person -->

    <owl:Class rdf:about="http://xmlns.com/foaf/0.1/Person">
        <rdfs:subClassOf rdf:resource="http://xmlns.com/foaf/0.1/Agent"/>
        <rdfs:comment>A person.</rdfs:comment>
        <rdfs:label>Person</rdfs:label>
    </owl:Class>
    


    <!-- 
    ///////////////////////////////////////////////////////////////////////////////////////
    //
    // General axioms
    //
    ///////////////////////////////////////////////////////////////////////////////////////
     -->

    <rdf:Description>
        <rdf:type rdf:resource="http://www.w3.org/2002/07/owl#AllDisjointClasses"/>
        <owl:members rdf:parseType="Collection">
            <rdf:Description rdf:about="http://purl.org/he/syllabus/ontology#Accessibility"/>
            <rdf:Description rdf:about="http://purl.org/he/syllabus/ontology#Attendance"/>
            <rdf:Description rdf:about="http://purl.org/he/syllabus/ontology#DropOut"/>
            <rdf:Description rdf:about="http://purl.org/he/syllabus/ontology#Qualification"/>
        </owl:members>
    </rdf:Description>
</rdf:RDF>



<!-- Generated by the OWL API (version 4.5.7.2018-12-02T02:23:35Z) https://github.com/owlcs/owlapi -->

